src/Datalog_Semantics.thy
@@ -1,0 +1,82 @@
+theory
+  Datalog_Semantics
+imports
+  Main
+  "~~/src/HOL/Library/Monad_Syntax"
+begin
+  
+subsection \<open>Semantics of Datalog rules\<close>
+
+datatype 'val element =
+  Var "string" |
+  Val "'val"
+
+datatype 'val atom =
+  Match "string" "'val element list"
+
+record 'val rule =
+  rule_rel    :: "string"
+  rule_params :: "string list"
+  rule_atoms  :: "'val atom set"
+
+type_synonym 'val fact = "string \<times> 'val list"
+type_synonym 'val database = "'val fact set"
+type_synonym 'val valuation = "string \<Rightarrow> 'val option"
+
+fun match_vars :: "'val element list \<Rightarrow> 'val list \<Rightarrow> 'val valuation option" where
+  "match_vars [] [] = Some Map.empty" |
+  "match_vars (Val x # vars) (val # vals) =
+     (if x = val then match_vars vars vals else None)" |
+  "match_vars (Var v # vars) (val # vals) = do {
+     mapping \<leftarrow> match_vars vars vals;
+     case mapping v of
+       None   \<Rightarrow> Some (mapping (v \<mapsto> val)) |
+       Some x \<Rightarrow> if x = val then Some mapping else None
+   }" |
+  "match_vars _ _ = None"
+
+fun subst_vars :: "'val element list \<Rightarrow> 'val valuation \<Rightarrow> 'val list option" where
+  "subst_vars [] mapping = Some []" |
+  "subst_vars (elem#vars) mapping = do {
+     values \<leftarrow> subst_vars vars mapping;
+     case elem of
+       Val x \<Rightarrow> Some (x#values) |
+       Var v \<Rightarrow> do { x \<leftarrow> mapping v; Some (x#values) }
+   }"
+
+definition match_atom :: "'val database \<Rightarrow> string \<Rightarrow> 'val element list \<Rightarrow> 'val database" where
+  "match_atom db rel vars \<equiv> {(rel',vars') \<in> db. rel = rel' \<and> match_vars vars vars' \<noteq> None}"
+
+fun satisfies :: "'val database \<Rightarrow> 'val atom \<Rightarrow> bool" (infix "\<Turnstile>" 60) where
+  "db \<Turnstile> Match rel vars = (match_atom db rel vars \<noteq> {})"
+
+thm match_vars.cases
+thm match_vars.elims
+thm match_vars.pelims
+thm match_vars.induct
+thm match_vars.simps
+find_theorems name: match_vars
+
+lemma match_vars_consistent:
+  assumes "match_vars vars vals = Some mapping"
+  shows "subst_vars vars mapping = Some vals"
+using assms apply(induction vars arbitrary: vals mapping)
+  apply(metis list.exhaust match_vars.simps(6) option.distinct(1) subst_vars.simps(1))
+  apply(subgoal_tac "\<exists>x vals'. vals = x#vals'", (erule exE)+, simp)
+  prefer 2
+  apply(metis list.exhaust match_vars.simps(5) option.distinct(1))
+  apply(erule_tac x="vals'" in meta_allE)
+  apply(subgoal_tac "\<exists>map'. match_vars vars vals' = Some map'", erule exE, simp)
+  prefer 2
+  apply(case_tac a, simp, meson bind_eq_Some_conv)
+  apply(metis match_vars.simps(2) option.discI)
+  apply(erule_tac x="map'" in meta_allE, simp)
+  apply(subgoal_tac "subst_vars vars map' = subst_vars vars mapping")
+  apply(case_tac a, simp)
+  apply(subgoal_tac "mapping x1 = Some x", simp)
+  apply(case_tac "map' x1", force)
+  apply(case_tac "aa = x", simp, simp)
+  apply(simp, metis option.simps(3))
+  oops
+
+end
